logrel and adequacy

src/adequacy.v
@@ -1,67 +1,55 @@
 From iris.program_logic Require Export adequacy.
-From iris_simp_lang Require Import simp heap_lib.
+From iris.proofmode Require Import proofmode.
+From iris.base_logic.lib Require Import ghost_map.
+From iris_simp_lang Require Import primitive_laws typing metatheory logrel.
+From iris_simp_lang Require Import lang.
 From iris.prelude Require Import options.
 
-(*|
-===========
-Adequacy
-===========
 
-This is a really important part of setting up the language. The infrastructure
-we've set up will let us prove specifications in Iris for simp_lang, but what do
-these theorems mean? This file proves **adequacy** of the weakest preconditions,
-which lifts a weakest precondition from within separation logic to a safety
-theorem about the semantics that's independent of Iris.
-
-Most of this is proven already for the generic weakest precondition definition
-we're using. Only one thing is missing: we need to initialize the state
-interpretation for the initial state. This gets to execute a ghost update, which
-we use to create the initial auth element for the heap_ra ghost state.
-
-The Coq implementation mostly consists of an orthogonal problem related to these
-Σ and related assumptions we make all over the place; if you want the details
-you should read
-https://gitlab.mpi-sws.org/iris/iris/-/blob/master/docs/resource_algebras.md,
-but here is a brief explanation. This argument is a list of RA functors and
-determine which ghost state is available in an Iris proof (this is needed to
-support impredicative ghost state, that is ghost state that refers to other
-ghost state). The simpGS assumption over Σ not only assumes that some RAs are
-available but also bundles a ghost name for the heap. Here, we allocate that
-ghost name and associated state.
-|*)
-
-(** These assumptions are just functors in Σ, unlike simpGS which also has a
-ghost name. *)
-Class simpGpreS Σ := SimpPreG {
-  simp_preG_iris :: invGpreS Σ;
-  simp_preG_heap :: heap_mapGpreS loc val Σ;
-}.
-
-Definition simpΣ : gFunctors :=
-  #[invΣ; heap_mapΣ loc val].
-
-Global Instance subG_heapGpreS {Σ} : subG simpΣ Σ → simpGpreS Σ.
+Global Instance subG_regGpreS Σ : subG regΣ Σ → regGpreS Σ.
 Proof. solve_inG. Qed.
 
-Lemma simp_adequacy Σ `{!simpGpreS Σ}
-           (s: stuckness) (e: expr) (σ: state) (φ: val → Prop) :
-  (∀ (simpGS0: simpGS Σ), ⊢ WP e @ s; ⊤ {{ v, ⌜φ v⌝ }}) →
-  adequate s e σ (λ (v: val) _, φ v).
+Definition init_state : state := {| heap := ∅; alive := ∅ |}.
+
+
+Lemma reg_adequacy Σ `{!regGpreS Σ, !invGpreS Σ}
+    (s : stuckness) (e : expr) (σ : state) (φ : val → Prop) :
+  (∀ (HregGS : regGS Σ), ⊢ WP e @ s; ⊤ {{ v, ⌜φ v⌝ }}) →
+  adequate s e σ (λ v _, φ v).
 Proof.
-  intros Hwp; eapply (wp_adequacy _ _); iIntros (??) "".
-  iMod (heap_map_init σ.(heap)) as (?) "Hh".
+  intros Hwp. apply (wp_adequacy Σ reg_lang). iIntros (Hinv κs) "".
+  iMod (ghost_map_alloc σ.(heap)) as (γh) "[Hh _]".
+  iMod (ghost_map_alloc σ.(alive)) as (γa) "[Ha _]".
   iModIntro.
-  iExists
-    (λ σ κs, (heap_map_interp σ.(heap))%I),
-    (λ _, True%I).
-  iFrame. iApply (Hwp (SimpGS _ _ _)).
+  iExists (λ σ' _, (ghost_map_auth γh 1 σ'.(heap) ∗
+                    ghost_map_auth γa 1 σ'.(alive))%I), (λ _, True%I).
+  iFrame "Hh Ha".
+  iApply (Hwp (@RegGS Σ Hinv _ _ γh γa)).
 Qed.
 
-(*|
-The thing to observe in the adequacy theorem's statement is that we assume
-`simpGpreS Σ` (these are just ordinary functors, which we'll get by including
-`simpΣ` in our definition of Σ) and then pass a `simpGS Σ` to a WP proof (this is
-higher-order, so you have to carefully follow the positive and negative
-occurrences). This is possible because `wp_adequacy` permits us to execute any
-initial ghost updates to create the first state interpretation.
-|*)
+Theorem sem_type_safety Σ `{!regGpreS Σ, !invGpreS Σ} e A :
+  (∀ (HregGS : regGS Σ), ⊢ ∅ ⊨ e : A @ ∅) →
+  adequate NotStuck e init_state (λ _ _, True).
+Proof.
+  intros Hsem. apply (reg_adequacy Σ). intros HregGS.
+  iPoseProof (Hsem HregGS) as "#H".
+  iSpecialize ("H" $! ∅ with "[]"); first iApply interp_env_empty.
+  iSpecialize ("H" $! ∅ with "[%] []").
+  { set_solver. }
+  { iApply live_empty. }
+  rewrite subst_map_empty.
+  iApply (wp_wand with "H"). by iIntros (v) "_".
+Qed.
+
+
+Theorem type_safe e A tp σ' e' :
+  typed ∅ e A ∅ →
+  rtc erased_step ([e], init_state) (tp, σ') →
+  e' ∈ tp →
+  not_stuck e' σ'.
+Proof.
+  intros Ht Hsteps Hin.
+  cut (adequate NotStuck e init_state (λ _ _, True)).
+  { intros [_ Hns]. by eapply Hns. }
+  apply (sem_type_safety regΣ e A). intros HregGS. by apply fundamental.
+Qed.
