src/proofmode.v
@@ -1,19 +1,14 @@
 From iris.proofmode Require Import coq_tactics reduction.
-From iris.proofmode Require Export tactics.
+From iris.proofmode Require Export proofmode.
 From iris.program_logic Require Import atomic.
-From iris_simp_lang Require Import tactics class_instances primitive_laws notation.
+From iris_simp_lang Require Import class_instances primitive_laws.
+From iris_simp_lang Require Export tactics.   
+From iris_simp_lang Require Import lang.
 From iris.prelude Require Import options.
 
-(*|
-This is a heavily stripped-down version of HeapLang's proofmode support. To make
-any program proofs reasonable we do need to implement `wp_pure` and `wp_bind`,
-and as a demo of the implementation we also implement `wp_load` in the
-reflective style typical in the IPM. `wp_pure` is the basis for a number of
-tactics like `wp_rec` and `wp_let` and such, while `wp_bind` is what powers
-`wp_apply`.
-|*)
 
-Lemma tac_wp_expr_eval `{!simpGS Σ} Δ s E Φ e e' :
+
+Lemma tac_wp_expr_eval `{!regGS Σ} Δ s E Φ e e' :
   (∀ (e'':=e'), e = e'') →
   envs_entails Δ (WP e' @ s; E {{ Φ }}) → envs_entails Δ (WP e @ s; E {{ Φ }}).
 Proof. by intros ->. Qed.
@@ -28,7 +23,7 @@ Tactic Notation "wp_expr_eval" tactic3(t) :=
   end.
 Ltac wp_expr_simpl := wp_expr_eval simpl.
 
-Lemma tac_wp_pure `{!simpGS Σ} Δ Δ' s E K e1 e2 φ n Φ :
+Lemma tac_wp_pure `{!regGS Σ} Δ Δ' s E K e1 e2 φ n Φ :
   PureExec φ n e1 e2 →
   φ →
   MaybeIntoLaterNEnvs n Δ Δ' →
@@ -42,11 +37,11 @@ Proof.
   iIntros "Hwp !> _" => //.
 Qed.
 
-Lemma tac_wp_value_nofupd `{!simpGS Σ} Δ s E Φ v :
+Lemma tac_wp_value_nofupd `{!regGS Σ} Δ s E Φ v :
   envs_entails Δ (Φ v) → envs_entails Δ (WP (Val v) @ s; E {{ Φ }}).
 Proof. rewrite envs_entails_unseal=> ->. by apply wp_value. Qed.
 
-Lemma tac_wp_value `{!simpGS Σ} Δ s E (Φ : val → iPropI Σ) v :
+Lemma tac_wp_value `{!regGS Σ} Δ s E (Φ : val → iPropI Σ) v :
   envs_entails Δ (|={E}=> Φ v) → envs_entails Δ (WP (Val v) @ s; E {{ Φ }}).
 Proof. rewrite envs_entails_unseal=> ->. by rewrite wp_value_fupd. Qed.
 
@@ -111,6 +106,7 @@ Ltac wp_pures :=
 (** Unlike [wp_pures], the tactics [wp_rec] and [wp_lam] should also reduce
 lambdas/recs that are hidden behind a definition, i.e. they should use
 [AsRecV_recv] as a proper instance instead of a [Hint Extern].
+  (* We want [pure_exec_fill] to be available to TC search locally. *)
 
 We achieve this by putting [AsRecV_recv] in the current environment so that it
 can be used as an instance by the typeclass resolution system. We then perform
@@ -121,20 +117,16 @@ Tactic Notation "wp_rec" :=
   wp_pure (App _ _);
   clear H.
 
-Tactic Notation "wp_if" := wp_pure (If _ _ _).
-Tactic Notation "wp_if_true" := wp_pure (If (LitV (LitBool true)) _ _).
-Tactic Notation "wp_if_false" := wp_pure (If (LitV (LitBool false)) _ _).
-Tactic Notation "wp_unop" := wp_pure (UnOp _ _).
-Tactic Notation "wp_binop" := wp_pure (BinOp _ _ _).
-Tactic Notation "wp_op" := wp_unop || wp_binop.
 Tactic Notation "wp_lam" := wp_rec.
 Tactic Notation "wp_let" := wp_pure (Rec BAnon (BNamed _) _); wp_lam.
 Tactic Notation "wp_seq" := wp_pure (Rec BAnon BAnon _); wp_lam.
-Tactic Notation "wp_proj" := wp_pure (Fst _) || wp_pure (Snd _).
 Tactic Notation "wp_pair" := wp_pure (Pair _ _).
+Tactic Notation "wp_proj" := wp_pure (Fst _) || wp_pure (Snd _).
+Tactic Notation "wp_inj" := wp_pure (InjL _) || wp_pure (InjR _).
+Tactic Notation "wp_case" := wp_pure (Case _ _ _ _ _).
 Tactic Notation "wp_closure" := wp_pure (Rec _ _ _).
 
-Lemma tac_wp_bind `{!simpGS Σ} K Δ s E Φ e f :
+Lemma tac_wp_bind `{!regGS Σ} K Δ s E Φ e f :
   f = (λ e, fill K e) → (* as an eta expanded hypothesis so that we can `simpl` it *)
   envs_entails Δ (WP e @ s; E {{ v, WP f (Val v) @ s; E {{ Φ }} }})%I →
   envs_entails Δ (WP fill K e @ s; E {{ Φ }}).
@@ -155,45 +147,6 @@ Tactic Notation "wp_bind" open_constr(efoc) :=
   | _ => fail "wp_bind: not a 'wp'"
   end.
 
-(*|
-=====================
-Convenience tactics
-=====================
-
-`wp_load` is just a shorthand for using the `wp_load` lemma.
-|*)
-
-
-(** Heap tactics *)
-Section heap.
-Context `{!simpGS Σ}.
-Implicit Types P Q : iProp Σ.
-Implicit Types Φ : val → iProp Σ.
-Implicit Types Δ : envs (uPredI (iResUR Σ)).
-Implicit Types (l: loc) (v : val) (z : Z).
-
-Lemma tac_wp_load Δ Δ' s E i K b (l: loc) v Φ :
-  MaybeIntoLaterNEnvs 1 Δ Δ' →
-  envs_lookup i Δ' = Some (b, l ↦ v)%I →
-  envs_entails Δ' (WP fill K (Val v) @ s; E {{ Φ }}) →
-  envs_entails Δ (WP fill K (Load (LitV l)) @ s; E {{ Φ }}).
-Proof.
-  rewrite envs_entails_unseal=> ?? Hi.
-  rewrite into_laterN_env_sound /=.
-  iIntros "Henv".
-  iDestruct (envs_lookup_split with "Henv") as "[Hl Henv]"; first by eauto.
-  iApply wp_bind.
-  destruct b; simpl.
-  - iDestruct "Hl" as ">#Hl".
-    iApply (wp_load with "Hl"). iIntros "!> _".
-    iApply Hi. iApply ("Henv" with "Hl").
-  - iDestruct "Hl" as ">Hl".
-    iApply (wp_load with "Hl"). iIntros "!> Hl".
-    iApply Hi. iApply ("Henv" with "Hl").
-Qed.
-
-End heap.
-
 (** Evaluate [lem] to a hypothesis [H] that can be applied, and then run
 [wp_bind K; tac H] for every possible evaluation context.  [tac] can do
 [iApplyHyp H] to actually apply the hypothesis.  TC resolution of [lem] premises
@@ -212,40 +165,3 @@ Tactic Notation "wp_apply_core" open_constr(lem) tactic3(tac) :=
     end).
 Tactic Notation "wp_apply" open_constr(lem) :=
   wp_apply_core lem (fun H => iApplyHyp H; try iNext; try wp_expr_simpl).
-
-Tactic Notation "wp_load" :=
-  let solve_pointsto _ :=
-    let l := match goal with |- _ = Some (_, (?l ↦ _)%I) => l end in
-    iAssumptionCore || fail "wp_load: cannot find" l "↦ ?" in
-  wp_pures;
-  lazymatch goal with
-  | |- envs_entails _ (wp ?s ?E ?e ?Q) =>
-    first
-      [reshape_expr e ltac:(fun K e' => eapply (tac_wp_load _ _ _ _ _ K))
-      |fail 1 "wp_load: cannot find 'Load' in" e];
-    [tc_solve
-    |solve_pointsto ()
-    |wp_finish]
-  | _ => fail "wp_load: not a 'wp'"
-  end.
-
-(* These tactics are not implemented reflectively out of laziness, but they do
-get the job done. Don't be afraid to implement helpers like this, though! They
-can be slightly buggier, slower, and give worse error messages but it's great
-for prototyping. *)
-
-Tactic Notation "wp_alloc" ident(l) "as" constr(H) :=
-  wp_apply (wp_alloc with "[//]"); iIntros (l) H.
-
-Tactic Notation "wp_store" :=
-  wp_pures;
-  wp_bind (Store _ _);
-  lazymatch goal with
-  | |- envs_entails ?Δ (wp ?s ?E (Store (Val (LitV (LitInt ?l))) _) ?Q) =>
-    lazymatch Δ with
-    | context[Esnoc _ ?i (l ↦ _)%I] =>
-      wp_apply (wp_store with i); iIntros i
-    | _ => fail "wp_store: could not find" l "↦ v"
-    end
-  | _ => fail "wp_store: not a 'wp'"
-  end.
