src/tactics.v
@@ -1,6 +1,6 @@
 From stdpp Require Import fin_maps.
 From iris_simp_lang Require Import lang.
-From iris Require Import options.
+From iris.prelude Require Import options.
 
 (*|
 This file implements some low-level tactics used to implement simp_lang.
@@ -13,24 +13,27 @@ proving typeclass instances that describe simp_lang's reduction rules.
 evaluation context [K] and a subexpression [e']. It calls the tactic [tac K e']
 for each possible decomposition until [tac] succeeds. *)
 Ltac reshape_expr e tac :=
-  (* Note that the current context is spread into a list of fully-constructed
-     items [K] A fully-constructed item is inserted into [K] by calling
-     [add_item]. *)
   let rec go K e :=
     match e with
-    | _                               => tac K e
-    | App ?e (Val ?v)                 => add_item (AppLCtx v) K e
-    | App ?e1 ?e2                     => add_item (AppRCtx e1) K e2
-    | UnOp ?op ?e                     => add_item (UnOpCtx op) K e
-    | BinOp ?op ?e (Val ?v)           => add_item (BinOpLCtx op v) K e
-    | BinOp ?op ?e1 ?e2               => add_item (BinOpRCtx op e1) K e2
-    | HeapOp ?op ?e (Val ?v)          => add_item (HeapOpLCtx op v) K e
-    | HeapOp ?op ?e1 ?e2              => add_item (HeapOpRCtx op e1) K e2
-    | If ?e0 ?e1 ?e2                  => add_item (IfCtx e1 e2) K e0
+    | _                          => tac K e
+    | App ?e (Val ?v)            => add_item (AppLCtx v) K e
+    | App ?e1 ?e2                => add_item (AppRCtx e1) K e2
+    | Pair ?e (Val ?v)           => add_item (PairLCtx v) K e
+    | Pair ?e1 ?e2               => add_item (PairRCtx e1) K e2
+    | Fst ?e                     => add_item FstCtx K e
+    | Snd ?e                     => add_item SndCtx K e
+    | InjL ?e                    => add_item InjLCtx K e
+    | InjR ?e                    => add_item InjRCtx K e
+    | Case ?e ?x1 ?e1 ?x2 ?e2    => add_item (CaseCtx x1 e1 x2 e2) K e
+    | Alloc ?r ?e                => add_item (AllocCtx r) K e
+    | Load ?e                    => add_item LoadCtx K e
+    | Store ?e (Val ?v)          => add_item (StoreLCtx v) K e
+    | Store ?e1 ?e2              => add_item (StoreRCtx e1) K e2
+    | EndRegion ?ρ ?e            => add_item (EndRegionCtx ρ) K e
     end
   with add_item Ki K e := go (Ki :: K) e
   in go (@nil ectx_item) e.
-
+  
 (** The tactic [inv_base_step] performs inversion on hypotheses of the shape
 [base_step]. The tactic will discharge head-reductions starting from values, and
 simplifies hypothesis related to conversions from and to values, and finite map
@@ -38,17 +41,9 @@ operations. This tactic is slightly ad-hoc and tuned for proving our lifting
 lemmas. *)
 Ltac inv_base_step :=
   repeat match goal with
-  | _ => progress simplify_map_eq/= (* simplify memory stuff *)
+  | _ => progress simplify_map_eq/=
   | H : to_val _ = Some _ |- _ => apply of_to_val in H
   | H : base_step ?e _ _ _ _ _ |- _ =>
-     try (is_var e; fail 1); (* inversion yields many goals if [e] is a variable
-     and should thus better be avoided. *)
+     try (is_var e; fail 1);
      inversion H; subst; clear H
   end.
-
-Create HintDb base_step.
-Global Hint Extern 0 (base_reducible _ _) => eexists _, _, _, _; simpl : base_step.
-
-(* [simpl apply] is too stupid, so we need extern hints here. *)
-Global Hint Extern 1 (base_step _ _ _ _ _ _) => econstructor : base_step.
-Global Hint Extern 0 (base_step (HeapOp AllocOp _ _) _ _ _ _ _) => apply alloc_fresh : base_step.
